Lift new hello world program

cakeml_connection/hello_ag32VerilogScript.sml
@@ -1,6 +1,6 @@
 open hardwarePreamble;
 
-open hello_ag32ProofTheory;
+open helloProofTheory;
 
 open verilogTheory verilogTypeTheory verilogTranslatorTheory moduleTranslatorTheory;
 open ag32MachineTheory ag32EqTheory ag32VerilogTheory;
@@ -16,13 +16,10 @@ val exit_code_0_def = Define `
  exit_code_0 vs fextv <=>
   erun fextv <| vars := vs |> (ArrayIndex (Var "R") [Const (w2ver (1w:word6))]) = INR (w2ver (0w:word32))`;
 
-(* Defined based on hello world program config *)
-val halt_addr_def = Define `
- halt_addr mem_start = mem_start + n2w (heap_size + 4 * LENGTH data + 2 * ffi_offset)`;
-
 (* Should be moved, and replaced by event-based definition... *)
 val ag32_is_halted_def = Define `
- ag32_is_halted fin mem_start <=> (mget_var fin "PC") = INR (w2ver (halt_addr mem_start))`;
+ ag32_is_halted fin mem_start <=>
+ (mget_var fin "PC") = INR (w2ver (hello_machine_config mem_start).halt_pc)`;
 
 val init_R_lift = Q.store_thm("init_R_lift",
  `!init hol_s s fext i.
@@ -53,7 +50,7 @@ val after_R_lift = Q.store_thm("after_R_lift",
 
 val external_memory_configured_def = Define`
  external_memory_configured fext start contents ⇔
-  fext.mem = contents start ∧
+  fext.mem = contents ∧
   byte_aligned start ∧
   w2n start + memory_size < dimword (:32)`;
 
@@ -61,24 +58,28 @@ val ag32_verilog_types_def = Define `
  ag32_verilog_types = relMtypes ++ ag32types`;
 
 val hello_verilog = Q.store_thm("hello_verilog",
- `!vstep fext fextv init mem_start.
+ `!vstep fext fextv init mem_start cl inp.
    vars_has_type init ag32_verilog_types ∧
    INIT_verilog (fext 0) init ∧
 
    vstep = mrun fextv computer init ∧
 
    is_lab_env fext_accessor_verilog vstep fext mem_start ∧
-   external_memory_configured (fext 0) mem_start hello_init_memory ∧
-   lift_fext fextv fext
-   ==>
+   external_memory_configured (fext 0) mem_start (hello_init_memory mem_start (cl, inp)) ∧
+   lift_fext fextv fext ∧
+
+   SUM (MAP strlen cl) + LENGTH cl ≤ cline_size ∧
+   wfcl cl ∧
+   LENGTH inp ≤ stdin_size ∧
+   2 ≤ maxFD
+   ⇒
    ?k fin.
     vstep k = INR fin /\
-    let
-     outs = MAP (\mem. get_print_string (mem_start, mem)) (fext k).io_events
-    in
-     ag32_is_halted fin mem_start ∧
-     outs ≼ hello_outputs ∧
-     (exit_code_0 fin (fextv k) ==> outs = hello_outputs)`,
+    let outs = MAP (get_ag32_io_event mem_start) (fext k).io_events;
+        outs_spec = MAP get_output_io_event (hello_io_events cl (stdin_fs inp)) in
+      ag32_is_halted fin mem_start ∧
+      outs ≼ outs_spec ∧
+      (exit_code_0 fin (fextv k) ⇒ (outs = outs_spec))`,
  rewrite_tac[external_memory_configured_def,ag32_verilog_types_def] \\
  rpt strip_tac \\
  drule_strip (vars_has_type_append |> SPEC_ALL |> EQ_IMP_RULE |> fst |> SPEC_ALL) \\
@@ -86,15 +87,15 @@ val hello_verilog = Q.store_thm("hello_verilog",
  drule_strip relM_backwards \\
  drule_strip INIT_backwards \\
  pop_assum (qspec_then `mem_start` strip_assume_tac) \\
+ qmatch_asmsub_abbrev_tac `INIT _ _ s'` \\
 
  drule_strip (GEN_ALL hello_ag32_next) \\
- qmatch_asmsub_abbrev_tac `INIT _ _ s'` \\
 
  `INIT_ISA s' mem_start` by (qunabbrev_tac `s'` \\ simp [INIT_ISA_def, combinTheory.UPDATE_APPLY]) \\
  disch_then (qspec_then `s'` mp_tac) \\
  impl_tac >-
  (qunabbrev_tac `s'` \\
-  fs [INIT_verilog_def, ag32_targetTheory.is_ag32_init_state_def, ag32Theory.print_string_max_length_def] \\
+  fs [INIT_verilog_def, ag32_targetTheory.is_ag32_init_state_def] \\
   match_mp_tac EQ_EXT \\
   rw [ag32_targetTheory.ag32_init_regs_def, combinTheory.UPDATE_APPLY] \\
   drule_strip init_R_lift \\ fs [] \\ metis_tac [combinTheory.UPDATE_APPLY]) \\
@@ -105,9 +106,10 @@ val hello_verilog = Q.store_thm("hello_verilog",
 
  drule_strip (SIMP_RULE (srw_ss()) [] INIT_REL_circuit_verilog) \\
  pop_assum(qspec_then`k1`strip_assume_tac) \\
- asm_exists_tac \\ fs [REL_def, hello_machine_config_def] \\ conj_tac
+ asm_exists_tac \\
+ fs [REL_def, ag32_is_halted_def, hello_machine_config_def, ag32_machine_config_def] \\ conj_tac
 
- >- fs [ag32_is_halted_def, relM_def, relM_var_def, WORD_def, halt_addr_def]
+ >- fs [relM_def, relM_var_def, WORD_def]
 
  \\ strip_tac \\ drule_strip after_R_lift \\ drule_first);
 
